unique_ids_loops.thy
@@ -1,0 +1,11 @@
+section "Unique Ids in loop programs"
+
+theory unique_ids_loops
+  imports program_proof_rules_loops
+begin
+
+text "We show that programs using the loop language are well formed with respect to unique identifiers."
+
+
+
+end
